fairneris/aneris_lang/state_interp/state_interp_config_wp.v
@@ -14,6 +14,8 @@ From fairneris.aneris_lang.state_interp Require Import
      state_interp_messages_history_coh
      state_interp_events
      state_interp_messages_history.
+From trillium.fairness Require Import fairness.
+From fairneris Require Import model_draft.
 
 From RecordUpdate Require Import RecordSet.
 Set Default Proof Using "Type".
@@ -22,7 +24,7 @@ Import uPred.
 Import RecordSetNotations.
 
 Section state_interpretation.
-  Context `{!anerisG Mdl Σ}.
+  Context `{!anerisG (fair_model_to_model simple_fair_model) Σ}.
 
   (* TODO: Move this elsehwere and use it where we now use ad hoc induction *)
   Lemma fupd_elim_laterN E1 E2 n (P:iProp Σ) :
@@ -36,10 +38,19 @@ Section state_interpretation.
     iApply ("IHn" with "HP Hclose").
   Qed.
 
+  Lemma elem_of_mABn m n : m ∈ mABn n → m = mAB.
+  Proof. induction n; set_solver. Qed.
+
+  Lemma elem_of_gset_of_gmultiset_gset `{Countable C} (M : gmultiset C) x :
+    x ∈ gset_of_gmultiset M ↔ x ∈ M.
+  Proof.
+    rewrite /gset_of_gmultiset gmultiset_elem_of_dom. apply elem_of_multiplicity.
+  Qed.
+
   Lemma config_wp_correct : ⊢ config_wp.
   Proof.
     rewrite /config_wp. iModIntro.
-    iIntros (ex atr c lbl σ2 Hexvalid Hex Hstep) "(Hevs & Hsi & Hm & % & Hauth)".
+    iIntros (ex atr c lbl σ2 Hexvalid Hex Hstep) "(Hevs & Hsi & % & Hauth)".
     rewrite (last_eq_trace_ends_in ex c); [|done].
     iDestruct "Hsi" as (γm mh)
                          "(%Hhist & %Hgcoh & %Hnscoh & %Hmhcoh &
@@ -47,44 +58,363 @@ Section state_interpretation.
     iMod (steps_auth_update_S with "Hauth") as "Hauth".
     iApply fupd_elim_laterN; [solve_ndisj|].
     destruct c as [tp1 σ1]=> /=.
-    iExists (trace_last atr), ().
-    rewrite (aneris_events_state_interp_same_tp _ (tp1, _));
-      [| |done|done]; last first.
-    { econstructor; [done| |done]. econstructor 2; eauto. }
-    iFrame "Hm Hevs Hauth Hsi".
-    iSplit; [|by iPureIntro; left].
-    iExists γm, mh. iFrame.
-    inversion Hstep as [ip σ Sn Sn' sh a skt R m Hm HSn Hsh HSn' Hsaddr|σ|σ];
-      simplify_eq/=.
-    - iSplit.
-      { apply (last_eq_trace_ends_in) in Hex as ->.
-        erewrite <- message_history_evolution_deliver_message;
-          eauto with set_solver. }
-      iSplitR; [eauto using gnames_coh_update_sockets|].
-      iSplitR; [eauto using network_sockets_coh_deliver_message|].
-      iSplitR; [iPureIntro; apply messages_history_coh_drop_message;
-                eauto using messages_history_coh_deliver_message|].
-      iSplitL "Hlcoh";
-        [by iApply (local_state_coh_deliver_message with "Hlcoh")|].
-      iApply free_ips_coh_ms. by iApply free_ips_coh_deliver_message.
-    - iFrame.
-      iSplit.
-      { iPureIntro.
-        simplify_eq /=.
-        apply (last_eq_trace_ends_in) in Hex as ->.
-        rewrite -message_history_evolution_duplicate_message; [done|].
-        by apply gmultiset_singleton_subseteq_l. }
-      iSplitR; [done|]. iSplitR; [done|].
-      iPureIntro. by apply messages_history_coh_duplicate_message.
-    - iFrame.
-      iSplit.
-      { iPureIntro.
-        simplify_eq /=.
-        apply (last_eq_trace_ends_in) in Hex as ->.
-        rewrite -message_history_evolution_drop_message; first done.
-        apply gmultiset_difference_subseteq. }
-      iSplitR; [done|]. iSplitR; [done|].
-      by iPureIntro; eapply messages_history_coh_drop_message.
+    rewrite /simple_valid_state_evolution in H.
+    rewrite /trace_ends_in in Hex.
+    rewrite Hex in H. simpl in *.
+    destruct σ1; simpl in *; simplify_eq.
+    destruct (trace_last atr).
+    { destruct H as [Hσ _].
+      inversion Hstep as [ip σ Sn Sn' sh a skt R m Hm HSn Hsh HSn' Hsaddr|σ|σ];
+        simplify_eq/=.
+      - rewrite /messages_to_receive_at_multi_soup in Hm. set_solver.
+      - set_solver.
+      - set_solver. }
+    (* Sent *)
+    - destruct H as [Hσ H'].
+      inversion Hstep as [ip σ Sn Sn' sh a skt R m Hm HSn Hsh HSn' Hsaddr|σ|σ];
+        simplify_eq/=.
+      (* Deliver *)
+      + destruct sent;
+          [by rewrite /messages_to_receive_at_multi_soup in Hm; set_solver|].
+        iExists (Delivered sent 1), (Some Ndeliver).
+        rewrite (aneris_events_state_interp_same_tp _ (tp1, _));
+          [| |done|done]; last first.
+        { econstructor; [done| |done]. econstructor 2; eauto. }
+        iFrame "Hevs Hauth Hsi".
+        iSplit; last first.
+        { iPureIntro.
+          rewrite /simple_valid_state_evolution.
+          rewrite /messages_to_receive_at_multi_soup in Hm.
+          assert (m = mAB) as ->.
+          { apply elem_of_filter in Hm as [Hdest Hm].
+            apply elem_of_gset_of_gmultiset_gset in Hm.
+            apply elem_of_mABn in Hm.
+            done. }
+          assert (a = m_destination mAB) as ->.
+          { by apply elem_of_filter in Hm as [-> _]. }
+          split; [multiset_solver|].
+          destruct H' as (shA & sh' & H').
+          exists shA, sh'.
+          assert (state_sockets0 !! ip = Some Sn) as HSn' by eauto.
+          apply Hnscoh in HSn as (?&?&?&?&?).
+          assert (ip = ip_of_address saB) as ->.
+          { eapply H2 in Hsh. eapply Hsh in Hsaddr. done. }
+          assert (Sn = {[sh' := (sB, mABm 0)]}) as ->.
+          { rewrite H' in HSn'.
+            rewrite insert_commute in HSn'; [|done].
+            rewrite lookup_insert in HSn'.
+            by inversion HSn'. }
+          assert (sh = sh') as ->.
+          { rewrite lookup_insert_Some in Hsh. set_solver. }
+          assert (skt = sB) as ->.
+          { rewrite lookup_insert in Hsh. set_solver. }
+          assert (R = []) as ->.
+          { rewrite lookup_insert in Hsh. set_solver. }
+          rewrite H'.
+          simpl.
+          rewrite insert_insert.
+          rewrite insert_commute; [|done]. rewrite insert_insert.
+          set_solver. }
+        iExists γm, mh. iFrame.
+        iSplit.
+        { apply (last_eq_trace_ends_in) in Hex as ->.
+          erewrite <- message_history_evolution_deliver_message;
+            eauto with set_solver. }
+        iSplitR; [eauto using gnames_coh_update_sockets|].
+        iSplitR; [eauto using network_sockets_coh_deliver_message|].
+        iSplitR; [iPureIntro; apply messages_history_coh_drop_message;
+                  eauto using messages_history_coh_deliver_message|].
+        iSplitL "Hlcoh";
+          [by iApply (local_state_coh_deliver_message with "Hlcoh")|].
+        by iApply (free_ips_coh_deliver_message with "Hfreeips").
+      (* Dup *)
+      + iExists (Sent $ S sent), (Some Ndup).
+        rewrite (aneris_events_state_interp_same_tp _ (tp1, _));
+          [| |done|done]; last first.
+        { econstructor; [done| |done]. econstructor 2; eauto. }
+        iFrame "Hevs Hauth Hsi".
+        iSplit; last first.
+        { iPureIntro.
+          rewrite /simple_valid_state_evolution.
+          apply elem_of_mABn in H as ->.
+          split; [done|done]. }
+        iExists γm, mh. iFrame.
+        iSplit.
+        { apply (last_eq_trace_ends_in) in Hex as ->.
+          erewrite <- message_history_evolution_duplicate_message;
+            eauto with set_solver.
+          by apply gmultiset_singleton_subseteq_l. }
+        iSplitR; [done|]. iSplitR; [done|].
+        iPureIntro. by apply messages_history_coh_duplicate_message.
+      (* Drop *)
+      + destruct sent as [|sent]; [by set_solver|].
+        iExists (Sent sent), (Some Ndrop).
+        rewrite (aneris_events_state_interp_same_tp _ (tp1, _));
+          [| |done|done]; last first.
+        { econstructor; [done| |done]. econstructor 2; eauto. }
+        iFrame "Hevs Hauth Hsi".
+        iSplit; last first.
+        { iPureIntro.
+          rewrite /simple_valid_state_evolution.
+          apply elem_of_mABn in H as ->. simpl.
+          split; [by multiset_solver|done]. }
+        iExists γm, mh. iFrame.
+        iSplit.
+        { iPureIntro.
+          simplify_eq /=.
+          apply (last_eq_trace_ends_in) in Hex as ->.
+          rewrite -message_history_evolution_drop_message; first done.
+          apply gmultiset_difference_subseteq. }
+        iSplitR; [done|]. iSplitR; [done|].
+        iPureIntro. by apply messages_history_coh_drop_message.
+    (* Delivered *)
+    - destruct H as [Hσ H'].
+      inversion Hstep as [ip σ Sn Sn' sh a skt R m Hm HSn Hsh HSn' Hsaddr|σ|σ];
+        simplify_eq/=.
+      (* Deliver *)
+      + destruct sent;
+          [by rewrite /messages_to_receive_at_multi_soup in Hm; set_solver|].
+        iExists (Delivered sent (S delivered)), (Some Ndeliver).
+        rewrite (aneris_events_state_interp_same_tp _ (tp1, _));
+          [| |done|done]; last first.
+        { econstructor; [done| |done]. econstructor 2; eauto. }
+        iFrame "Hevs Hauth Hsi".
+        iSplit; last first.
+        { iPureIntro.
+          rewrite /simple_valid_state_evolution.
+          rewrite /messages_to_receive_at_multi_soup in Hm.
+          assert (m = mAB) as ->.
+          { apply elem_of_filter in Hm as [_ Hm].
+            apply elem_of_gset_of_gmultiset_gset in Hm.
+            apply elem_of_mABn in Hm.
+            done. }
+          assert (a = m_destination mAB) as ->.
+          { by apply elem_of_filter in Hm as [-> _]. }
+          split; [multiset_solver|].
+          destruct H' as (shA & sh' & H').
+          exists shA, sh'.
+          assert (state_sockets0 !! ip = Some Sn) as HSn' by eauto.
+          apply Hnscoh in HSn as (?&?&?&?&?).
+          assert (ip = ip_of_address saB) as ->.
+          { eapply H2 in Hsh. eapply Hsh in Hsaddr. done. }
+          assert (Sn = {[sh' := (sB, mABm delivered)]}) as ->.
+          { rewrite H' in HSn'.
+            rewrite insert_commute in HSn'; [|done].
+            rewrite lookup_insert in HSn'.
+            by inversion HSn'. }
+          assert (sh = sh') as ->.
+          { rewrite lookup_insert_Some in Hsh. set_solver. }
+          assert (skt = sB) as ->.
+          { rewrite lookup_insert in Hsh. set_solver. }
+          assert (R = mABm delivered) as ->.
+          { rewrite lookup_insert in Hsh. set_solver. }
+          rewrite H'.
+          simpl.
+          rewrite insert_insert.
+          rewrite insert_commute; [|done]. rewrite insert_insert. 
+          set_solver. }
+        iExists γm, mh. iFrame.
+        iSplit.
+        { apply (last_eq_trace_ends_in) in Hex as ->.
+          erewrite <- message_history_evolution_deliver_message;
+            eauto with set_solver. }
+        iSplitR; [eauto using gnames_coh_update_sockets|].
+        iSplitR; [eauto using network_sockets_coh_deliver_message|].
+        iSplitR; [iPureIntro; apply messages_history_coh_drop_message;
+                  eauto using messages_history_coh_deliver_message|].
+        iSplitL "Hlcoh";
+          [by iApply (local_state_coh_deliver_message with "Hlcoh")|].
+        by iApply (free_ips_coh_deliver_message with "Hfreeips").
+      (* Dup *)
+      + iExists (Delivered (S sent) delivered), (Some Ndup).
+        rewrite (aneris_events_state_interp_same_tp _ (tp1, _));
+          [| |done|done]; last first.
+        { econstructor; [done| |done]. econstructor 2; eauto. }
+        iFrame "Hevs Hauth Hsi".
+        iSplit; last first.
+        { iPureIntro.
+          rewrite /simple_valid_state_evolution.
+          apply elem_of_mABn in H as ->.
+          split; [done|done]. }
+        iExists γm, mh. iFrame.
+        iSplit.
+        { apply (last_eq_trace_ends_in) in Hex as ->.
+          erewrite <- message_history_evolution_duplicate_message;
+            eauto with set_solver.
+          by apply gmultiset_singleton_subseteq_l. }
+        iSplitR; [done|]. iSplitR; [done|].
+        iPureIntro. by apply messages_history_coh_duplicate_message.
+      (* Drop *)
+      + destruct sent as [|sent]; [by set_solver|].
+        iExists (Delivered sent delivered), (Some Ndrop).
+        rewrite (aneris_events_state_interp_same_tp _ (tp1, _));
+          [| |done|done]; last first.
+        { econstructor; [done| |done]. econstructor 2; eauto. }
+        iFrame "Hevs Hauth Hsi".
+        iSplit; last first.
+        { iPureIntro.
+          rewrite /simple_valid_state_evolution.
+          apply elem_of_mABn in H as ->. simpl.
+          split; [by multiset_solver|done]. }
+        iExists γm, mh. iFrame.
+        iSplit.
+        { iPureIntro.
+          simplify_eq /=.
+          apply (last_eq_trace_ends_in) in Hex as ->.
+          rewrite -message_history_evolution_drop_message; first done.
+          apply gmultiset_difference_subseteq. }
+        iSplitR; [done|]. iSplitR; [done|].
+        iPureIntro. by apply messages_history_coh_drop_message.
+    (* Delivered *)
+    - destruct H as [Hσ H'].
+      inversion Hstep as [ip σ Sn Sn' sh a skt R m Hm HSn Hsh HSn' Hsaddr|σ|σ];
+        simplify_eq/=.
+      (* Deliver *)
+      + destruct sent;
+          [by rewrite /messages_to_receive_at_multi_soup in Hm; set_solver|].
+        iExists (Received sent (S delivered)), (Some Ndeliver).
+        rewrite (aneris_events_state_interp_same_tp _ (tp1, _));
+          [| |done|done]; last first.
+        { econstructor; [done| |done]. econstructor 2; eauto. }
+        iFrame "Hevs Hauth Hsi".
+        iSplit; last first.
+        { iPureIntro.
+          rewrite /simple_valid_state_evolution.
+          rewrite /messages_to_receive_at_multi_soup in Hm.
+          assert (m = mAB) as ->.
+          { apply elem_of_filter in Hm as [Hdest Hm].
+            apply elem_of_gset_of_gmultiset_gset in Hm.
+            apply elem_of_mABn in Hm.
+            done. }
+          assert (a = m_destination mAB) as ->.
+          { by apply elem_of_filter in Hm as [-> _]. }
+          simpl.
+          split; [multiset_solver|].
+          destruct H' as (shA & sh' & H').
+          exists shA, sh'.
+          assert (state_sockets0 !! ip = Some Sn) as HSn' by eauto.
+          apply Hnscoh in HSn as (?&?&?&?&?).
+          assert (ip = ip_of_address saB) as ->.
+          { eapply H2 in Hsh. eapply Hsh in Hsaddr. done. }
+          assert (Sn = {[sh' := (sB, mABm delivered)]}) as ->.
+          { rewrite H' in HSn'.
+            rewrite insert_commute in HSn'; [|done].
+            rewrite lookup_insert in HSn'.
+            by inversion HSn'. }
+          assert (sh = sh') as ->.
+          { rewrite lookup_insert_Some in Hsh. set_solver. }
+          assert (skt = sB) as ->.
+          { rewrite lookup_insert in Hsh. set_solver. }
+          assert (R = mABm delivered) as ->.
+          { rewrite lookup_insert in Hsh. set_solver. }
+          rewrite H'.
+          simpl.
+          rewrite insert_insert.
+          rewrite insert_commute; [|done]. rewrite insert_insert. 
+          set_solver. }
+        iExists γm, mh. iFrame.
+        iSplit.
+        { apply (last_eq_trace_ends_in) in Hex as ->.
+          erewrite <- message_history_evolution_deliver_message;
+            eauto with set_solver. }
+        iSplitR; [eauto using gnames_coh_update_sockets|].
+        iSplitR; [eauto using network_sockets_coh_deliver_message|].
+        iSplitR; [iPureIntro; apply messages_history_coh_drop_message;
+                  eauto using messages_history_coh_deliver_message|].
+        iSplitL "Hlcoh";
+          [by iApply (local_state_coh_deliver_message with "Hlcoh")|].
+        by iApply (free_ips_coh_deliver_message with "Hfreeips").
+      (* Dup *)
+      + iExists (Received (S sent) delivered), (Some Ndup).
+        rewrite (aneris_events_state_interp_same_tp _ (tp1, _));
+          [| |done|done]; last first.
+        { econstructor; [done| |done]. econstructor 2; eauto. }
+        iFrame "Hevs Hauth Hsi".
+        iSplit; last first.
+        { iPureIntro.
+          rewrite /simple_valid_state_evolution.
+          apply elem_of_mABn in H as ->.
+          split; [done|done]. }
+        iExists γm, mh. iFrame.
+        iSplit.
+        { apply (last_eq_trace_ends_in) in Hex as ->.
+          erewrite <- message_history_evolution_duplicate_message;
+            eauto with set_solver.
+          by apply gmultiset_singleton_subseteq_l. }
+        iSplitR; [done|]. iSplitR; [done|].
+        iPureIntro. by apply messages_history_coh_duplicate_message.
+      (* Drop *)
+      + destruct sent as [|sent]; [by set_solver|].
+        iExists (Received sent delivered), (Some Ndrop).
+        rewrite (aneris_events_state_interp_same_tp _ (tp1, _));
+          [| |done|done]; last first.
+        { econstructor; [done| |done]. econstructor 2; eauto. }
+        iFrame "Hevs Hauth Hsi".
+        iSplit; last first.
+        { iPureIntro.
+          rewrite /simple_valid_state_evolution.
+          apply elem_of_mABn in H as ->. simpl.
+          split; [by multiset_solver|done]. }
+        iExists γm, mh. iFrame.
+        iSplit.
+        { iPureIntro.
+          simplify_eq /=.
+          apply (last_eq_trace_ends_in) in Hex as ->.
+          rewrite -message_history_evolution_drop_message; first done.
+          apply gmultiset_difference_subseteq. }
+        iSplitR; [done|]. iSplitR; [done|].
+        iPureIntro. by apply messages_history_coh_drop_message.
   Qed.
+
+  (* Lemma config_wp_correct : ⊢ config_wp. *)
+  (* Proof. *)
+  (*   rewrite /config_wp. iModIntro. *)
+  (*   iIntros (ex atr c lbl σ2 Hexvalid Hex Hstep) "(Hevs & Hsi & Hm & % & Hauth)". *)
+  (*   rewrite (last_eq_trace_ends_in ex c); [|done]. *)
+  (*   iDestruct "Hsi" as (γm mh) *)
+  (*                        "(%Hhist & %Hgcoh & %Hnscoh & %Hmhcoh & *)
+  (*                          Hnauth & Hsi & Hlcoh & Hfreeips & Hmctx & Hmres)". *)
+  (*   iMod (steps_auth_update_S with "Hauth") as "Hauth". *)
+  (*   iApply fupd_elim_laterN; [solve_ndisj|]. *)
+  (*   destruct c as [tp1 σ1]=> /=. *)
+  (*   iExists (trace_last atr), (). *)
+  (*   rewrite (aneris_events_state_interp_same_tp _ (tp1, _)); *)
+  (*     [| |done|done]; last first. *)
+  (*   { econstructor; [done| |done]. econstructor 2; eauto. } *)
+  (*   iFrame "Hm Hevs Hauth Hsi". *)
+  (*   iSplit; [|by iPureIntro; left]. *)
+  (*   iExists γm, mh. iFrame. *)
+  (*   inversion Hstep as [ip σ Sn Sn' sh a skt R m Hm HSn Hsh HSn' Hsaddr|σ|σ]; *)
+  (*     simplify_eq/=. *)
+  (*   - iSplit. *)
+  (*     { apply (last_eq_trace_ends_in) in Hex as ->. *)
+  (*       erewrite <- message_history_evolution_deliver_message; *)
+  (*         eauto with set_solver. } *)
+  (*     iSplitR; [eauto using gnames_coh_update_sockets|]. *)
+  (*     iSplitR; [eauto using network_sockets_coh_deliver_message|]. *)
+  (*     iSplitR; [iPureIntro; apply messages_history_coh_drop_message; *)
+  (*               eauto using messages_history_coh_deliver_message|]. *)
+  (*     iSplitL "Hlcoh"; *)
+  (*       [by iApply (local_state_coh_deliver_message with "Hlcoh")|]. *)
+  (*     iApply free_ips_coh_ms. by iApply free_ips_coh_deliver_message. *)
+  (*   - iFrame. *)
+  (*     iSplit. *)
+  (*     { iPureIntro. *)
+  (*       simplify_eq /=. *)
+  (*       apply (last_eq_trace_ends_in) in Hex as ->. *)
+  (*       rewrite -message_history_evolution_duplicate_message; [done|]. *)
+  (*       by apply gmultiset_singleton_subseteq_l. } *)
+  (*     iSplitR; [done|]. iSplitR; [done|]. *)
+  (*     iPureIntro. by apply messages_history_coh_duplicate_message. *)
+  (*   - iFrame. *)
+  (*     iSplit. *)
+  (*     { iPureIntro. *)
+  (*       simplify_eq /=. *)
+  (*       apply (last_eq_trace_ends_in) in Hex as ->. *)
+  (*       rewrite -message_history_evolution_drop_message; first done. *)
+  (*       apply gmultiset_difference_subseteq. } *)
+  (*     iSplitR; [done|]. iSplitR; [done|]. *)
+  (*     by iPureIntro; eapply messages_history_coh_drop_message. *)
+  (* Qed. *)
 
 End state_interpretation.
